Slew of updates.  Hankin 2 & 3 now build with either basis.  Have made a start on generating labelled terms by doing quotient.  Fitting it into existing proofs may be tricky.  Will likely drop existing GM approach to this (in gmltermScript.ml) as it's hideous.

examples/lambda/binderLib.sig
@@ -9,7 +9,7 @@ sig
   val recursive_term_function_existence : term -> thm
   val prove_recursive_term_function_exists : term -> thm
   val define_recursive_term_function :
-      term quotation -> thm * thm option
+      term quotation -> thm * thm
 
   (* stores recursion theorems for types *)
   val type_db : (string,thm) Binarymap.dict ref
